process/inversion.v
@@ -5,6 +5,13 @@ From mathcomp Require Import ssreflect.seq.
 Import ListNotations.
 From Paco Require Import paco.
 
+Lemma empty_nil: forall {A: Type} (l: list A),
+  0 = length l <-> l = [].
+Proof. intros A l.
+       case l; intros; easy.
+Qed.
+   
+
 Lemma zip_eq: forall {A B: Type} (l1 l3: list A) (l2 l4: list B),
   length l1 = length l2 -> length l2 = length l3 -> length l3 = length l4 ->
   (zip l1 l2) = (zip l3 l4) ->
@@ -51,97 +58,57 @@ Proof. intros A B l1.
          apply IHl1. easy.
 Qed.
 
-Lemma _a23_a: forall em p L Q P Gs Gt T, 
+Lemma remove_S : forall {a b : fin}, S a = S b -> a = b.
+Proof.
+  intros.
+  inversion H. easy.
+Qed.
+
+Lemma _a23_a: forall em p lb pr L Q P Gs Gt T, 
   typ_proc em Gs Gt P T ->
-  P = (p_recv p (zip L Q)) -> 
-  (exists T' S, length T' = length L -> length T' = length S -> length T' = length Q -> subtypeC (ltt_recv p (zip (zip L S) T')) T /\  
+  P = (p_recv p (zip (lb::L) (pr::Q))) -> 
+  (exists ty st T' S, length (ty::T') = length (lb::L) -> length (ty::T') = length (st::S) -> length (ty::T') = length (pr::Q) -> subtypeC (ltt_recv p (zip (zip (lb::L) (st::S)) (ty::T'))) T /\  
+  typ_proc (Datatypes.S em) (extendS Gs em st) Gt pr ty /\
   List.Forall (fun u => typ_proc (Datatypes.S em) (extendS Gs em (fst u)) Gt (fst (snd u)) (snd (snd u))) (zip S (zip Q T'))).
 Proof. intros.
        induction H; intros; try easy.
        specialize(IHtyp_proc H0).
-       destruct IHtyp_proc as (T',IHtyp_proc).
-       exists T'.
-       simpl.
-       destruct IHtyp_proc as [S'].
-       exists S'.
-       intros Hla1 Hla2 Hla3.
-       split.
-       specialize(H4 Hla1 Hla2 Hla3).
-       destruct H4 as (IHtyp_proc, Ha).
-       specialize(stTrans (ltt_recv p (zip (zip L S') T')) t t' IHtyp_proc); intro HT.
-       apply HT.
+       destruct IHtyp_proc as (q',IHtyp_proc).
+       destruct IHtyp_proc. destruct H2. destruct H2. simpl in H2.
+       exists q'. exists x. exists x0. exists x1. simpl.
+       intros.
+       specialize(H2 H3 H4 H5); intros.
+       destruct H2. destruct H6. split.
+       specialize(stTrans (ltt_recv p ((lb, x, q') :: zip (zip L x1) x0)) t t' H2 H1); intros.
        easy.
-       
-       (**)
-       destruct H4 as (IHtyp_proc, Ha). easy. easy. easy.
+       split. easy.
        apply Forall_forall.
-       intros (x1,(x2,x3)) Hx.
+       intros (y1, (y2, y3)) Hx.
        simpl in *.
-       rewrite Forall_forall in Ha.
-       specialize(Ha (x1,(x2,x3))). simpl in Ha.
-       specialize(tc_sub (Datatypes.S em) (extendS cs em x1) (extendS cs' em x1) ct ct' x2 x3 x3); intro HTC.
-       apply HTC.
-(*        specialize(tc_sub m (Datatypes.S em) c); intro HTC. *)
-       apply Ha. easy.
-       apply stRefl.
-       simpl. 
-       specialize(leq_consS cs cs' em x1 x1 (srefl x1) H2); intros. easy. easy.
-     
-       exists T. exists ST.
-       intros Hla1 Hla2 Hla3.
-       split.
-       inversion H0. subst.
-       assert(length (zip L0 ST) = length L0) as Hasrt1.
-       { symmetry.
-         apply zip_len. easy.
-       }
+       rewrite Forall_forall in H7.
+       specialize(H7 (y1,(y2,y3)) Hx); intros. 
+       simpl in H7. easy.
+       
+       clear IHtyp_proc.
+       inversion H0. subst. 
+       exists ty. exists st. exists T. exists ST.
+       intros. simpl in *.
+       specialize(remove_S H5); intros. 
+       specialize(remove_S H6); intros. 
+       specialize(remove_S H7); intros.
+       clear H5 H6 H7. 
+       
        assert(L0 = L /\ P = Q).
        { 
           specialize(eq_trans H H1); intros.
-          specialize(eq_trans H2 Hla1); intros.
-          specialize(eq_trans (eq_sym Hla1) Hla3); intros.
-          specialize(zip_eq L0 L P Q H4 H5 H7 H6); intros.
+          specialize(eq_trans H2 H8); intros.
+          specialize(eq_trans (eq_sym H8) H11); intros.
+          specialize(zip_eq L0 L P Q H5 H6 H7 H9); intros.
           easy.
        }
-       subst.
-       pfold.
-       destruct H4.
-       replace L0 with L.
-       apply sub_in. easy. easy.
-       clear H H1 H2 H3 H6 Hla1 Hla2 Hla3 Hasrt1.
-       apply Forall_forall.
-       intros (x1,x2) Hx.
-       induction ST; intros.
-       simpl in Hx. easy.
-       simpl in Hx.
-       destruct Hx as [Hx | Hx].
-       inversion Hx. subst.
-       simpl. apply srefl.
-       simpl. apply IHST. easy. 
-
-       apply Forall_forall.
-       intros (x1,x2) Hx.
-       clear H H1 H2 H3 Hla1 Hla2 Hla3 Hasrt1.
-       induction T; intros.
-       simpl in Hx. easy.
-       simpl in Hx.
-       simpl in IHT.
-       destruct Hx as [Hx | Hx].
-       inversion Hx. subst. simpl.
-       specialize(stRefl x2); intro HT.
-       punfold HT. apply st_mon.
-       simpl. apply IHT. easy.
-       inversion H0.
-       assert(L0 = L /\ P = Q).
-       { 
-          specialize(eq_trans H H1); intros.
-          specialize(eq_trans H2 Hla1); intros.
-          specialize(eq_trans (eq_sym Hla1) Hla3); intros.
-          specialize(zip_eq L0 L P Q H4 H7 H8 H6); intros.
-          easy.
-       }
-       destruct H4. 
-       replace Q with P.
+       destruct H5. subst.
+       split. easy.
+       split. easy.
        easy.
 Qed.
 
@@ -151,16 +118,16 @@ Lemma _a23_b: forall em p l e Q P Gs Gt T,
   P = (p_send p l e Q) -> exists S S' T', typ_expr Gs e S /\ typ_proc em Gs Gt Q T' /\ subsort S' S /\ subtypeC (ltt_send p [(l,S',T')]) T.
 Proof. intros em p l e Q P Gs Gt T H.
        induction H; intros; try easy.
-       specialize(IHtyp_proc H3).
+       specialize(IHtyp_proc H1).
        destruct IHtyp_proc as (S,(S',(T',Ha))).
        exists S. exists S'. exists T'.
        split.
-       specialize(sc_sub cs cs' e S S); intro HSS.
-       apply HSS. easy. apply srefl. easy.
+       specialize(sc_sub cs e S S); intro HSS.
+       apply HSS. easy. apply srefl. 
        split.
-       specialize(tc_sub em cs cs' ct ct' Q T' T'); intro HTS.
+       specialize(tc_sub em cs ct Q T' T'); intro HTS.
        apply HTS. easy.
-       apply stRefl. easy. easy. split. easy.
+       apply stRefl. split. easy.
        destruct Ha as (Ha,(Hb,(Hc,Hd))).
        specialize(stTrans (ltt_send p [(l, S', T')]) t t' Hd H0); intro HT.
        apply HT.
@@ -201,31 +168,26 @@ Proof. intros.
        destruct IHtyp_proc as (T1,(T2,(Ha,(Hb,(Hc,Hd))))).
        exists T1. exists T2.
        split.
-       specialize(tc_sub em cs cs' ct ct' Q1 T1 T1); intro HTS.
-       apply HTS. easy. apply stRefl. easy. easy.
-       split.
-       specialize(tc_sub em cs cs' ct ct' Q2 T2 T2); intro HTS.
-       apply HTS. easy. apply stRefl. easy. easy. 
-       split.
+       specialize(tc_sub em cs ct Q1 T1 T1); intro HTS.
+       apply HTS. easy. apply stRefl. split. easy. split. 
        specialize(stTrans T1 t t' Hc H1); intro HT. easy.
        specialize(stTrans T2 t t' Hd H1); intro HT. easy.
 Qed.
 
 Lemma _a23_d: forall P em x Q T Gs Gt,
   typ_proc em Gs Gt P T ->
-  P = (p_rec x Q)   -> typ_proc em Gs (extendT Gt x T) Q T.
+  P = (p_rec x Q)   -> exists T', (typ_proc em Gs (extendT Gt x T') Q T' /\ subtypeC T' T).
 Proof. intros.
        induction H; intros; try easy.
        inversion H0. subst.
-       unfold ct' in *. easy.
-
-       subst.
-       apply tc_sub with
-       (ct := extendT ct x t) (cs := cs) (t := t).
-       apply IHtyp_proc. easy.
-       easy. easy.
-       specialize(leq_consT ct ct' x t t' H1 H3); intros. easy.
-Qed.
+       exists t. split. easy. easy.
+       specialize(IHtyp_proc H0). 
+       destruct IHtyp_proc. exists x0. destruct H2.
+       split.
+       easy.
+       specialize(stTrans x0 t t' H3 H1); intros. easy.
+Qed. 
+(* 
 
 Lemma helper_a23_e_1 : forall x X n l x0 ct t, (Some t = lookupT ct X) -> (leq_ctxT (extendT x0 X x) ct) -> ((X =? n)%nat = false)
     -> subtypeC x t -> leq_ctxT (consT X x (consT n l x0)) (consT n l ct).
@@ -264,50 +226,180 @@ Proof.
   apply emptyT.
   apply 0.
   
+Qed. *)
+
+Lemma refl_eq_ctxT : forall m, consistent_ctxT m -> eq_ctxT m m.
+Proof.
+  intros. 
+  unfold eq_ctxT. intros.
+  split. easy. split. easy.
+  induction lookupT. easy. easy.
+Qed.
+
+Lemma band_destruct : forall (a b : bool), true = a -> true = b -> true = (a && b)%bool.
+Proof.
+  intros. destruct H0. replace a with true. easy.
+Qed.
+
+Lemma bnat_comm : forall a b, ((a =? b)%nat = (b =? a)%nat).
+Proof. 
+      intros.
+      specialize(Nat.eqb_eq a b); intros.
+      specialize(Nat.eqb_eq b a); intros.
+      specialize(Nat.eqb_neq a b); intros.
+      specialize(Nat.eqb_neq b a); intros.
+      case_eq (a =? b)%nat.
+      - intros.
+        destruct H. specialize(H H3). 
+        specialize(eq_sym H); intros.
+        destruct H0. specialize(H6 H5). 
+        replace (b =? a)%nat with true.
+        easy.
+      - intros. destruct H1. specialize(H1 H3); intros.
+        specialize(not_eq_sym H1); intros.
+        destruct H2. specialize(H6 H5); intros. easy.
+Qed.
+
+Lemma swap_eq_ctxT : forall m X Y T T', consistent_ctxT (consT X T (consT Y T' m)) -> eq_ctxT (consT X T (consT Y T' m)) (consT Y T' (consT X T m)).
+Proof.
+  intros.
+  unfold eq_ctxT. intros.
+  split. easy. split. 
+  assert(consistent_ctxT (consT Y T' (consT X T m))).
+  {
+    simpl in H.
+    simpl.
+    case_eq (Nat.eqb X Y); intros.
+    replace (X =? Y)%nat with true in H. destruct H. easy.
+    replace (X =? Y)%nat with false in H.
+    specialize(bnat_comm Y X); intros.
+    specialize(eq_trans H1 H0); intros. 
+    replace (Y =? X)%nat with false.
+    split. destruct H. destruct H3.
+    easy. destruct H. destruct H3. split. easy. easy.
+  }
+  easy.
+  simpl. simpl in H.
+  case_eq (Nat.eqb n X); intros. 
+  - case_eq (Nat.eqb n Y); intros; try easy.
+    specialize(Nat.eqb_eq n X); intros. destruct H2. specialize(H2 H0); intros.
+    specialize(Nat.eqb_eq n Y); intros. destruct H4. specialize(H4 H1); intros.
+    specialize(eq_sym H2); intros. specialize(eq_trans H6 H4); intros.
+    specialize(Nat.eqb_eq X Y); intros. destruct H8. specialize(H9 H7); intros.
+    replace (X =? Y)%nat with true in H. simpl in H. easy.
+  - case_eq (Nat.eqb n Y); intros. try easy.
+    easy.
+Qed.
+
+Lemma sym_eq_ctxT : forall m1 m2, eq_ctxT m1 m2 -> eq_ctxT m2 m1.
+Proof.
+  intros.
+  unfold eq_ctxT in *.
+  intros.
+  specialize(H n); intros.
+  destruct H. destruct H0.
+  split. easy. split. easy. easy.
+Qed.
+
+Lemma trans_eq_ctxT : forall m1 m2 m3, 
+      eq_ctxT m1 m2 -> eq_ctxT m2 m3 -> eq_ctxT m1 m3.
+Proof.
+  intros.
+  unfold eq_ctxT in *.
+  intros.
+  split. specialize(H n); intros. easy. split. specialize(H0 n); intros. easy.
+  specialize(H n); intros.
+  specialize(H0 n); intros. 
+  destruct H0. destruct H1. destruct H. destruct H3. 
+  specialize(eq_trans H4 H2); intros. easy.
+Qed.
+  
+Lemma cons_eq_ctxT_helper : forall m1 m2 n, eq_ctxT m1 m2 -> lookupT m1 n = None -> lookupT m2 n = None.
+Proof. 
+  intros.
+  unfold eq_ctxT in H. specialize(H n); intros.
+  destruct H. destruct H1.
+  specialize(eq_trans (eq_sym H2) H0); intros.
+  easy.
+Qed.
+
+Lemma cons_eq_ctxT : forall m1 m2 n T, eq_ctxT m1 m2 -> lookupT m1 n = None -> eq_ctxT (consT n T m1) (consT n T m2).
+Proof.
+  intros.
+  pose proof H as H1.
+  unfold eq_ctxT. intros.
+  specialize(H n0); intros. destruct H. destruct H2. 
+  split.
+  simpl. split. easy. easy.
+  split. simpl. split. 
+  specialize(cons_eq_ctxT_helper m1 m2 n H1 H0); intros.
+  easy. easy.
+  simpl. 
+  case_eq (n0 =? n)%nat; intros; try easy.
 Qed.
 
 Lemma _a23_e: forall P em X T Gs Gt,
   typ_proc em Gs Gt P T ->
-  (P = (p_var X) -> exists T' G', leq_ctxT (extendT G' X T') Gt /\ subtypeC T' T).
+  (P = (p_var X) -> exists T' G', eq_ctxT (extendT G' X T') Gt /\ subtypeC T' T).
 Proof. intros.
        induction H; intros; try easy.
        inversion H0. subst.
-       induction ct; intros. easy.
-       simpl in H.
        
-       case_eq (Nat.eqb X n); intros Hb.
+       induction ct. simpl in H2. easy.
+       simpl in H2.
+       case_eq (Nat.eqb X n); intros.
+       replace (X =? n)%nat with true in H2. inversion H2.
+       simpl in H1. destruct H1.
+       specialize(IHct H4); intros.
+       unfold extendT in *.
+       exists l. exists ct. split; try easy.
+       specialize(natb_to_prop X n H3); intros. replace X with n. easy.
        
-       replace (X =? n)%nat with true in H.
-       inversion H. 
-       exists l. exists ct. unfold extendT. 
+       replace (X =? n)%nat with false in H2.
+       simpl in H1. destruct H1. 
+       specialize(IHct H4 H2); intros.
+       destruct IHct. destruct H5.
+       exists x. exists (extendT x0 n l).
+       unfold extendT in *.
+       destruct H5.
+       specialize(sym_eq_ctxT (consT X x x0) ct H5); intros.
+       specialize(cons_eq_ctxT ct (consT X x x0) n l H7 H1); intros.
+       Compute (swap_eq_ctxT).
+       specialize(swap_eq_ctxT x0 X n x l); intros.
+       specialize(sym_eq_ctxT (consT n l ct) (consT n l (consT X x x0))); intros.
+       
+       simpl in H9. replace (X =? n)%nat with false in H9. 
+       assert(lookupT x0 X = None /\ lookupT x0 n = None /\ consistent_ctxT x0).
+       {
+         split; try easy. 
+         unfold eq_ctxT in H5. simpl in H5.
+         specialize(H5 n); intros. destruct H5. destruct H5.
+         easy. split.
+         
+         unfold eq_ctxT in H8. simpl in H8.
+         specialize(bnat_comm n X ); intros. specialize(eq_trans H11 H3); intros.
+         replace (n =? X)%nat with false in H8.
+         specialize(H8 n); intros. destruct H8. destruct H13. destruct H13. easy.
+         
+         unfold eq_ctxT in H5. specialize(H5 n); intros. simpl in H5.
+         destruct H5. destruct H5. easy.
+       }
+       specialize(H9 H11); intros.
+       specialize(sym_eq_ctxT (consT X x (consT n l x0)) (consT n l (consT X x x0)) H9); intros.
+       specialize(trans_eq_ctxT (consT n l ct) (consT n l (consT X x x0)) (consT X x (consT n l x0)) H8 H12); intros.
        split. 
-       specialize(natb_to_prop X n Hb); intros.
-       subst.
-       apply leq_ctxT_refl.
-       easy.
-
-       replace (X =? n)%nat with false in H.
-       specialize(IHct H).
-       destruct IHct. destruct H1.
-       exists x. exists (consT n l x0).
-       split. unfold extendT.
-       destruct H1.
-       specialize(helper_a23_e_1 x X n l x0 ct t H H1 Hb H2); intros.
-       easy.
-       
-       destruct H1.
-       easy.
-       
-       specialize(IHtyp_proc H0).
-       destruct IHtyp_proc. destruct H4.
-(*        specialize(ref_stronger_T ct ct' H3); intros. *)
-       destruct H4.
-       specialize(leq_ctxT_trans (extendT x0 X x) ct ct' H4 H3); intros.
-       specialize(stTrans x t t' H5 H1); intros.
-       exists x. exists x0.
-       split.
+       specialize(sym_eq_ctxT (consT n l ct) (consT X x (consT n l x0)) H13); intros.
        easy. easy.
+       
+       specialize(IHtyp_proc H0); intros.
+       destruct IHtyp_proc. destruct H2.
+       exists x. exists x0. 
+       destruct H2. split.
+       easy.
+       specialize(stTrans x t t' H3 H1); intros.
+       easy.
 Qed.
+       
 
 Lemma _a23_f: forall P em T Gs Gt,
   typ_proc em Gs Gt P T ->
