process/substitution.v
@@ -1,0 +1,113 @@
+From SST Require Import aux.unscoped aux.expressions process.processes process.typecheck process.inversion type.global tree.global tree.local.
+Require Import List String Datatypes ZArith Relations PeanoNat.
+Open Scope list_scope.
+From mathcomp Require Import ssreflect.seq.
+Import ListNotations.
+From Paco Require Import paco.
+
+Lemma _typ_consistency_ : forall em Gs Gt P T, typ_proc em Gs Gt P T -> (consistent_ctxS Gs /\ consistent_ctxT Gt).
+intros.
+  induction H; intros; try easy.
+  destruct IHtyp_proc.
+  split; try easy.
+  simpl in H1. destruct H1. easy.
+  destruct IHtyp_proc.
+  simpl in H4. destruct H4.
+  split. easy. easy.
+Qed.
+
+Lemma trivial_type_inact : forall em Gs Gt T, typ_proc em Gs Gt p_inact T -> T = ltt_end.
+Proof.
+  intros. 
+  specialize(_a23_f p_inact em T Gs Gt H (eq_refl p_inact)); intros.
+  easy.
+Qed.
+
+Lemma remove_unusedT_inact : forall em Gs Gt X T T',
+  typ_proc em Gs (extendT Gt X T) p_inact T' -> typ_proc em Gs Gt p_inact T'.
+Proof.
+  intros.
+  specialize(trivial_type_inact em Gs (extendT Gt X T) T' H); intros. subst.
+  specialize(tc_inact em Gs Gt); intros.
+  specialize(_typ_consistency_ em Gs (extendT Gt X T) p_inact ltt_end H); intros.
+  destruct H1. simpl in H2. destruct H2.
+  specialize(H0 H1 H3); intros.
+  easy.
+Qed.
+
+Lemma remove_unusedT_var : forall em Gs Gt X Y T T',
+  Y <> X -> typ_proc em Gs (extendT Gt X T) (p_var Y) T' -> typ_proc em Gs Gt (p_var Y) T'.
+Proof.
+  intros.
+  specialize(_a23_e (p_var Y) em Y T' Gs (extendT Gt X T) H0 (eq_refl (p_var Y))); intros.
+  destruct H1. destruct H1. destruct H1.
+  unfold eq_ctxT in H1.
+  specialize(H1 Y); intros. simpl in H1.
+  destruct H1. destruct H1. destruct H3. destruct H3.
+  specialize(Nat.eqb_refl Y); intros.
+  replace (Y =? Y)%nat with true in H5.
+  specialize(Nat.eqb_neq Y X); intros. destruct H8. specialize(H9 H); intros.
+  replace (Y =? X)%nat with false in H5.
+  
+  specialize(tc_var em Gs Gt Y x); intros.
+  specialize(_typ_consistency_ em Gs (extendT Gt X T) (p_var Y) T' H0); intros.
+  destruct H11. simpl in H12. destruct H12.
+  specialize(H10 H11 H13 H5); intros.
+  specialize(tc_sub em Gs Gt (p_var Y) x T' H10 H2); intros.
+  easy.
+Qed.
+
+Lemma _a21: forall P Q em T Gs Gt X Q',
+  typ_proc em Gs (extendT Gt X T) P T -> typ_proc em Gs Gt Q T 
+  -> substitutionP (p_var X) Q P Q'
+  -> typ_proc em Gs Gt Q' T.
+Proof. 
+  intro P.
+  induction P.
+  (* var *)
+  intros.
+  inversion H1. subst. easy. subst. 
+  specialize(_a23_e (p_var n) em n T Gs (extendT Gt X T) H (eq_refl (p_var n))); intros.
+  specialize(not_eq_sym H5); intros.
+  specialize(remove_unusedT_var em Gs Gt X n T T H3 H); intros. easy.
+  subst. inversion H3.
+  
+  (* inact *) 
+  intros.
+  specialize (_a23_f p_inact em T Gs (extendT Gt X T) H (eq_refl p_inact)); intros.
+  subst.
+  inversion H1; intros; try easy.
+  subst.
+  specialize(_typ_consistency_ em Gs Gt Q ltt_end H0); intros.
+  destruct H2.
+  specialize(tc_inact em Gs Gt H2 H3); intros. easy.
+    
+  (* send *)
+  intros. 
+  specialize(_a23_b em s n e P (p_send s n e P) Gs (extendT Gt X T) T H (eq_refl (p_send s n e P))); intros.
+  destruct H2. destruct H2. destruct H2. destruct H2. destruct H3. destruct H4.
+  
+(*   inversion H1; intros; try easy. 
+  
+  subst.
+  specialize(tc_send); intros. *)
+  
+  
+  
+  
+  admit.
+  (* recv *) 
+  admit.
+  
+  (* ite *)
+  intros.   
+  admit.
+  
+  (* mu *)
+  intros. 
+  specialize(_a23_d); intros.
+  
+  admit.
+   
+Admitted.
+
